<rdf:RDF
    xmlns:rdf="http://www.w3.org/1999/02/22-rdf-syntax-ns#"
    xmlns:schema="https://schema.org/"
    xmlns:vs="http://www.w3.org/2003/06/sw-vocab-status/ns#"
    xmlns:dbo="http://dbpedia.org/ontology/"
    xmlns:voaf="http://purl.org/vocommons/voaf#"
    xmlns:rdfs="http://www.w3.org/2000/01/rdf-schema#"
    xmlns:bot="https://w3id.org/bot#"
    xmlns:dce="http://purl.org/dc/elements/1.1/"
    xmlns:dcterms="http://purl.org/dc/terms/"
    xmlns:owl="http://www.w3.org/2002/07/owl#"
    xmlns:vcard="http://www.w3.org/2006/vcard/ns#"
    xmlns:vann="http://purl.org/vocab/vann/"
    xmlns:foaf="http://xmlns.com/foaf/0.1/"
    xmlns:xsd="http://www.w3.org/2001/XMLSchema#" > 
  <rdf:Description rdf:about="https://schema.org/domainIncludes">
    <rdf:type rdf:resource="http://www.w3.org/2002/07/owl#AnnotationProperty"/>
  </rdf:Description>
  <rdf:Description rdf:about="https://w3id.org/bot#Element">
    <rdfs:label xml:lang="nl">Gebouwelement</rdfs:label>
    <rdfs:isDefinedBy rdf:resource="https://w3id.org/bot#"/>
    <rdfs:comment xml:lang="sv">Beståndsdel av ett byggnadsverk med en karaktäristisk teknisk funktion, form eller position [12006-2, 3.4.7]</rdfs:comment>
    <rdfs:comment xml:lang="fr">Constituant d'un bâtiment remplissant une fonction technique spécifique ou ayant une forme ou une position spécifiques</rdfs:comment>
    <rdfs:label xml:lang="es">Elemento arquitectónico</rdfs:label>
    <rdfs:comment xml:lang="es">Componente de una construcción con una función técnica, forma o posición característica</rdfs:comment>
    <owl:disjointWith rdf:resource="https://w3id.org/bot#Interface"/>
    <rdfs:label xml:lang="de">Bauteil (Bauwesen)</rdfs:label>
    <rdfs:comment xml:lang="en">Constituent of a construction entity with a characteristic technical function, form or position [12006-2, 3.4.7]</rdfs:comment>
    <rdfs:label xml:lang="fr">Elément d'un bâtiment</rdfs:label>
    <rdfs:comment xml:lang="nl">Bestanddeel van een gebouwde entiteit met een karakteristieke technische functie, vorm of positie [12006-2, 3.4.7]</rdfs:comment>
    <rdfs:label xml:lang="sv">Byggdel</rdfs:label>
    <owl:disjointWith rdf:resource="https://w3id.org/bot#Zone"/>
    <rdf:type rdf:resource="http://www.w3.org/2002/07/owl#Class"/>
    <rdfs:label xml:lang="en">Building element</rdfs:label>
    <vs:term_status>stable</vs:term_status>
    <rdfs:comment xml:lang="da">Bestanddel af et bygværk med en karakteristisk funktion, form eller position [12006-2, 3.4.7]</rdfs:comment>
    <rdfs:label xml:lang="it">Elemento architettonico</rdfs:label>
    <rdfs:label xml:lang="da">Bygningsdel</rdfs:label>
    <rdfs:comment xml:lang="de">Das Bauteil ist im Bauwesen ein einzelnes Teil, ein Element oder eine Komponente, aus denen ein Bauwerk zusammengesetzt wird [12006-2, 3.4.7]</rdfs:comment>
  </rdf:Description>
  <rdf:Description rdf:nodeID="A0">
    <rdf:rest rdf:resource="http://www.w3.org/1999/02/22-rdf-syntax-ns#nil"/>
    <rdf:first rdf:resource="https://w3id.org/bot#hasElement"/>
  </rdf:Description>
  <rdf:Description rdf:about="https://schema.org/rangeIncludes">
    <rdf:type rdf:resource="http://www.w3.org/2002/07/owl#AnnotationProperty"/>
  </rdf:Description>
  <rdf:Description rdf:about="http://xmlns.com/foaf/0.1/name">
    <rdf:type rdf:resource="http://www.w3.org/2002/07/owl#DatatypeProperty"/>
  </rdf:Description>
  <rdf:Description rdf:about="https://w3id.org/bot#hasStorey">
    <rdfs:label xml:lang="sv">har våning</rdfs:label>
    <rdfs:comment xml:lang="fr">Relation à définir entre les étages d'une même zone. Cette propriété s'applique typiquement sur des instances de bot:Building.</rdfs:comment>
    <vs:term_status>stable</vs:term_status>
    <rdfs:label xml:lang="fr">a étage</rdfs:label>
    <rdfs:label xml:lang="es">tiene piso</rdfs:label>
    <rdfs:domain rdf:resource="https://w3id.org/bot#Zone"/>
    <rdfs:label xml:lang="de">hat Geschoss</rdfs:label>
    <rdfs:comment xml:lang="nl">Relatie tot de verdiepingen die zich in een zone bevinden. De typische domeinen van bot:hasStorey zijn instanties van bot:Building</rdfs:comment>
    <rdfs:label xml:lang="en">has storey</rdfs:label>
    <rdf:type rdf:resource="http://www.w3.org/2002/07/owl#ObjectProperty"/>
    <rdfs:subPropertyOf rdf:resource="https://w3id.org/bot#containsZone"/>
    <rdfs:isDefinedBy rdf:resource="https://w3id.org/bot#"/>
    <rdfs:range rdf:resource="https://w3id.org/bot#Storey"/>
    <schema:domainIncludes rdf:resource="https://w3id.org/bot#Building"/>
    <rdfs:comment xml:lang="de">Beziehung zwischen Geschossen, die in einer Zone enthalten sind. Oft ist die rdfs:domain eine Instanz von bot:Building.</rdfs:comment>
    <rdfs:label xml:lang="nl">heeft verdieping</rdfs:label>
    <rdfs:label xml:lang="da">har etage</rdfs:label>
    <rdfs:comment xml:lang="da">Relation til etager indeholdt i en zone. De typiske domæner for bot:hasStorey er forekomster af bot:Building.</rdfs:comment>
    <rdfs:comment xml:lang="en">Relation to storeys contained in a zone. The typical domains of bot:hasStorey are instances of bot:Building.</rdfs:comment>
  </rdf:Description>
  <rdf:Description rdf:about="https://w3id.org/bot#Site">
    <rdfs:comment xml:lang="en">Area containing one or more buildings.</rdfs:comment>
    <rdfs:isDefinedBy rdf:resource="https://w3id.org/bot#"/>
    <rdfs:subClassOf rdf:resource="https://w3id.org/bot#Zone"/>
    <owl:disjointWith rdf:resource="https://w3id.org/bot#Space"/>
    <rdfs:comment xml:lang="da">Område som indeholder en eller flere bygninger.</rdfs:comment>
    <rdfs:label xml:lang="es">Sitio</rdfs:label>
    <rdfs:label xml:lang="de">Grundstück</rdfs:label>
    <rdfs:label xml:lang="da">Grund</rdfs:label>
    <rdfs:comment xml:lang="fr">Un site comprend un ou plusieurs bâtiments</rdfs:comment>
    <rdf:type rdf:resource="http://www.w3.org/2002/07/owl#Class"/>
    <rdfs:label xml:lang="fr">Site</rdfs:label>
    <rdfs:label xml:lang="en">Site</rdfs:label>
    <rdfs:comment xml:lang="sv">En plats som rymmer en eller flera byggnader.</rdfs:comment>
    <vs:term_status>stable</vs:term_status>
    <rdfs:comment xml:lang="nl">Omgeving die één of meerdere gebouwen bevat.</rdfs:comment>
    <owl:disjointWith rdf:resource="https://w3id.org/bot#Building"/>
    <owl:disjointWith rdf:resource="https://w3id.org/bot#Storey"/>
    <rdfs:comment xml:lang="de">Abgegrenzter Teil der Erdoberfläche auf dem ein oder mehrere Gebäude stehen.</rdfs:comment>
    <rdfs:comment xml:lang="es">Área que contiene uno o más edificios.</rdfs:comment>
    <rdfs:label xml:lang="sv">Plats</rdfs:label>
    <rdfs:label xml:lang="nl">Terrein</rdfs:label>
  </rdf:Description>
  <rdf:Description rdf:nodeID="A1">
    <rdf:rest rdf:resource="http://www.w3.org/1999/02/22-rdf-syntax-ns#nil"/>
    <rdf:first rdf:resource="https://w3id.org/bot#containsElement"/>
  </rdf:Description>
  <rdf:Description rdf:about="https://w3id.org/bot#intersectsZone">
    <schema:domainIncludes rdf:resource="https://w3id.org/bot#Building"/>
    <rdfs:range rdf:resource="https://w3id.org/bot#Zone"/>
    <owl:propertyDisjointWith rdf:resource="https://w3id.org/bot#adjacentZone"/>
    <rdfs:comment xml:lang="en">Relationship between two zones whose 3D extent intersect. For example, a stairwell intersects different storeys.</rdfs:comment>
    <rdf:type rdf:resource="http://www.w3.org/2002/07/owl#ObjectProperty"/>
    <rdf:type rdf:resource="http://www.w3.org/2002/07/owl#SymmetricProperty"/>
    <schema:rangeIncludes rdf:resource="https://w3id.org/bot#Space"/>
    <rdfs:comment xml:lang="de">Beziehung zwischen zwei Zonen, die sich schneiden. Zum Beispiel schneidet eine Treppe verschiedene Geschosse.</rdfs:comment>
    <rdfs:label xml:lang="en">intersects zone</rdfs:label>
    <schema:domainIncludes rdf:resource="https://w3id.org/bot#Site"/>
    <schema:rangeIncludes rdf:resource="https://w3id.org/bot#Building"/>
    <rdfs:domain rdf:resource="https://w3id.org/bot#Zone"/>
    <schema:rangeIncludes rdf:resource="https://w3id.org/bot#Site"/>
    <schema:domainIncludes rdf:resource="https://w3id.org/bot#Space"/>
    <schema:rangeIncludes rdf:resource="https://w3id.org/bot#Storey"/>
    <rdfs:isDefinedBy rdf:resource="https://w3id.org/bot#"/>
    <rdfs:label xml:lang="de">sich schneidende Zone</rdfs:label>
    <vs:term_status>stable</vs:term_status>
    <schema:domainIncludes rdf:resource="https://w3id.org/bot#Storey"/>
  </rdf:Description>
  <rdf:Description rdf:about="http://purl.org/vocab/vann/preferredNamespacePrefix">
    <rdf:type rdf:resource="http://www.w3.org/2002/07/owl#AnnotationProperty"/>
  </rdf:Description>
  <rdf:Description rdf:about="http://purl.org/dc/terms/creator">
    <rdf:type rdf:resource="http://www.w3.org/2002/07/owl#AnnotationProperty"/>
  </rdf:Description>
  <rdf:Description rdf:about="http://purl.org/dc/terms/contributor">
    <rdf:type rdf:resource="http://www.w3.org/2002/07/owl#AnnotationProperty"/>
  </rdf:Description>
  <rdf:Description rdf:about="https://w3id.org/bot#hasElement">
    <rdfs:range rdf:resource="https://w3id.org/bot#Element"/>
    <rdfs:label xml:lang="nl">hoster element</rdfs:label>
    <rdfs:label xml:lang="nl">heeft element</rdfs:label>
    <rdf:type rdf:resource="http://www.w3.org/2002/07/owl#ObjectProperty"/>
    <rdfs:comment xml:lang="de">Beziehung zwischen einer Zone und einem Bauteil, dass entweder in der Zone enthalten ist, oder sich mit ihr schneidet. Diese Beziehung sollte nicht explizit benutzt werden, sondern ergibt sich implizit aus den Unterbeziehungen. Es ermöglicht, zum Beispiel, dass mit einer Abfrage alle Türen eines Gebäudes, die sich mit einer Zone schneiden ermittelt werden können.</rdfs:comment>
    <rdfs:comment xml:lang="en">Links a Zone to an Element that is either contained in or adjacent to, the Zone. The intended use of this relationship is not to be stated explicitly, but to be inferred from its sub-properties. It will, for example, allow one to query for all the doors of a building given that they have an adjacency to spaces of the building.</rdfs:comment>
    <owl:propertyChainAxiom rdf:nodeID="A2"/>
    <rdfs:domain rdf:resource="https://w3id.org/bot#Zone"/>
    <rdfs:comment xml:lang="da">Forbinder en Zone til en bygningsdel der enten er indeholdt i eller tilstødende til zonen. Det er ikke hensigten at denne relation angives eksplicit, men at den udledes af dennes underegneskaber. Det vil for eksempel tillade en forespørgsel på alle døre i en bygning givet at disse er enten tilstødende eller indeholdt i rum i bygningen.</rdfs:comment>
    <rdfs:isDefinedBy rdf:resource="https://w3id.org/bot#"/>
    <rdfs:label xml:lang="es">alberga elemento</rdfs:label>
    <rdfs:label xml:lang="fr">a élément</rdfs:label>
    <rdfs:label xml:lang="de">hat Bauteil</rdfs:label>
    <rdfs:label xml:lang="da">har element</rdfs:label>
    <rdfs:label xml:lang="sv">värd för element</rdfs:label>
    <vs:term_status>stable</vs:term_status>
    <rdfs:label xml:lang="en">has element</rdfs:label>
  </rdf:Description>
  <rdf:Description rdf:about="https://w3id.org/bot#Interface">
    <rdfs:comment xml:lang="nl">Een interface is een vlak waar twee gebouwelementen, twee zones of een gebouw elementen en een zone elkaar raken. Het kan worden gebruikt om de verbinding tussen de twee te kwalificeren. Een use case kan de kwalificatie van het warmteoverbrengingsoppervlak tussen een zone en een muur over meerdere zones zijn.</rdfs:comment>
    <rdfs:comment xml:lang="da">En grænseflade er fladen hvor to bygningsdele, to zoner eller en bygningsdel og en zone mødes. Den kan benyttes til at kvalificere forbindelsen mellem de to. En use case kunne være kvalifikation af varmetransmissionsarealet mellem en zone og en væg som dækker flere zoner.</rdfs:comment>
    <rdfs:isDefinedBy rdf:resource="https://w3id.org/bot#"/>
    <rdfs:label xml:lang="de">Grenzfläche</rdfs:label>
    <owl:disjointWith rdf:resource="https://w3id.org/bot#Zone"/>
    <vs:term_status>stable</vs:term_status>
    <rdfs:comment xml:lang="fr">Une interface correspond à la surface où se rencontrent a) deux éléments d'un bâtiment, b) deux zones ou  encore c) un élément d'un bâtiment avec une zone. Un cas d'utilisation type est constituée par la qualification de la zone de transmission de chaleur entre une zone et un mur couvrant plusieurs zones.</rdfs:comment>
    <rdfs:label xml:lang="da">Grænseflade</rdfs:label>
    <rdf:type rdf:resource="http://www.w3.org/2002/07/owl#Class"/>
    <rdfs:label xml:lang="sv">Gränssnitt</rdfs:label>
    <rdfs:comment xml:lang="de">Eine Grenzfläche ist die Fläche, an der sich zwei Bauteile, zwei Zonen oder ein Bauteil und eine Zone treffen. Das Konzept kann verwendet werden, um die Beziehung zwischen den Beteiligten zu qualifizieren. Ein Beispiel ist die Qualifizierung der Wärmeaustauschfläche zwischen eine Zone und einer Wand, die mehrere Zonen überdeckt.</rdfs:comment>
    <rdfs:comment xml:lang="sv">Ett gränssnitt är den yta där två byggdelar, två zoner eller en b yggdel och en zon möts. Det kan användas för att beskriva kopplingen mellan de två. Ett användningsfall kan vara att kvalificera värmetransmissionsarean mellan en zon och en vägg som täcker flera zoner.</rdfs:comment>
    <rdfs:comment xml:lang="en">An interface is the surface where two building elements, two zones or a building element and a zone meet. It can be used for qualification of the connection between the two. A use case could be qualification of the heat transmission area between a zone and a wall covering several zones.</rdfs:comment>
    <owl:disjointWith rdf:resource="https://w3id.org/bot#Element"/>
    <rdfs:label xml:lang="fr">Interface</rdfs:label>
    <rdfs:label xml:lang="nl">Interface</rdfs:label>
    <rdfs:label xml:lang="en">Interface</rdfs:label>
  </rdf:Description>
  <rdf:Description rdf:about="https://w3id.org/bot#hasSubElement">
    <rdfs:label xml:lang="de">hat Unterbauteil</rdfs:label>
    <rdf:type rdf:resource="http://www.w3.org/2002/07/owl#ObjectProperty"/>
    <rdfs:comment xml:lang="sv">Relation mellan en byggdel a) och en annan byggdel b) som utgör värd a). Exempel: inst:wall bot:hasSubElement inst:window</rdfs:comment>
    <rdfs:label xml:lang="nl">heeft sub element</rdfs:label>
    <rdfs:label xml:lang="da">hoster sub element</rdfs:label>
    <rdfs:label xml:lang="nl">hoster sub element</rdfs:label>
    <rdfs:comment xml:lang="en">Relation between an element a) and another element b) hosted by element a)</rdfs:comment>
    <rdfs:label xml:lang="es">alberga sub elemento</rdfs:label>
    <rdfs:comment xml:lang="da">Relation mellem en bygningsdel a) og en anden bygningsdel b) hostet af element a). Eksempel: inst:wall bot:hasSubElement inst:window</rdfs:comment>
    <rdfs:label xml:lang="fr">a sous-élément</rdfs:label>
    <rdfs:label xml:lang="en">has sub-element</rdfs:label>
    <rdfs:comment xml:lang="de">Beziehung zwischen einem Bauteil und a) einem anderen Bauteil oder b) einem Bauteil, dass ein anderes Bauteil enthält.</rdfs:comment>
    <rdfs:isDefinedBy rdf:resource="https://w3id.org/bot#"/>
    <rdfs:comment xml:lang="nl">Relatie tussen een gebouwelement a) en een ander element b) dat een ander element in zich heeft a). Voorbeeld: inst:wall bot:hasSubElement inst:window</rdfs:comment>
    <rdfs:domain rdf:resource="https://w3id.org/bot#Element"/>
    <rdfs:comment xml:lang="fr">Relation entre un élément du bâti A et un autre élément du bâti, B, contenu ou abrité dans A</rdfs:comment>
    <vs:term_status>stable</vs:term_status>
    <rdfs:range rdf:resource="https://w3id.org/bot#Element"/>
    <rdfs:label xml:lang="sv">värd för sub element</rdfs:label>
  </rdf:Description>
  <rdf:Description rdf:about="https://w3id.org/bot#has3DModel">
    <rdfs:label xml:lang="de">hat 3D Modell</rdfs:label>
    <rdfs:comment xml:lang="de">Verbindet eine Instanz von bot:Zone oder bot:Element zu einer IRI, die das zugehörige 3D Modell identifiziert. Das Modell kann in einem spezifischen RDF Vokabular kodiert sein. Andernfalls kann die IRI auch dereferenzierbar sein.</rdfs:comment>
    <schema:domainIncludes rdf:resource="https://w3id.org/bot#Element"/>
    <rdf:type rdf:resource="http://www.w3.org/2002/07/owl#ObjectProperty"/>
    <vs:term_status>unstable</vs:term_status>
    <rdfs:label xml:lang="en">has 3D Model</rdfs:label>
    <schema:domainIncludes rdf:resource="https://w3id.org/bot#Zone"/>
    <rdfs:comment xml:lang="da">Forbinder enhver instans af bot:Zone eller bot:Element med en IRI som identificerer dennes 3D-model. Denne 3D-model kan så beskrives ved brug af et dedikeret RDF-vokabular. Alternativt kan 3D-modellens IRI være dereferencerbar, sådan at der modtages en repræsentation af 3D-modellen i et eksisterende dataformat for 3D-modeller når IRIen slås op.</rdfs:comment>
    <rdfs:label xml:lang="da">har 3D-model</rdfs:label>
    <rdfs:isDefinedBy rdf:resource="https://w3id.org/bot#"/>
    <rdfs:comment xml:lang="en">Links any bot:Zone or bot:Element to a IRI that identifies its 3D Model. This 3D Model can then be described using some dedicated RDF vocabulary. Else, the 3D Model IRI could be dereferenceable, and when looking up the IRI one could retrieve a representation of the 3D Model with some existing data format for 3D models.</rdfs:comment>
  </rdf:Description>
  <rdf:Description rdf:about="https://orcid.org/0000-0002-6519-7057">
    <schema:name>Mads Holten Rasmussen</schema:name>
    <vcard:fn>Mads Holten Rasmussen</vcard:fn>
    <rdf:type rdf:resource="https://schema.org/Person"/>
    <rdf:type rdf:resource="http://www.w3.org/2006/vcard/ns#Individual"/>
  </rdf:Description>
  <rdf:Description rdf:about="http://purl.org/vocommons/voaf#Vocabulary">
    <rdf:type rdf:resource="http://www.w3.org/2002/07/owl#Class"/>
  </rdf:Description>
  <rdf:Description rdf:about="https://w3id.org/bot#hasZeroPoint">
    <rdfs:label xml:lang="de">hat Nullpunkt</rdfs:label>
    <rdfs:comment xml:lang="de">Verbindet eine Instanz von bot:Site mit einer Instanz, die den Längen- und Breitengrad des Nullpunkts des Grundstücks definiert. Dies kann eine Instanz eines wgs84:Point sein. Die Definition von GIS und Geometrie ist nicht Bestandteil von BOT. Die Nutzung dieses Properties ist potenziell zweideutig und es besteht die Möglichkeit das es in Zukunft überarbeitet oder entfernt wird.</rdfs:comment>
    <rdfs:label xml:lang="da">har nulpunkt</rdfs:label>
    <rdfs:seeAlso rdf:resource="https://github.com/w3c-lbd-cg/bot/issues/41"/>
    <rdfs:domain rdf:resource="https://w3id.org/bot#Site"/>
    <vs:term_status>unstable</vs:term_status>
    <rdfs:label xml:lang="en">has zero point</rdfs:label>
    <rdfs:isDefinedBy rdf:resource="https://w3id.org/bot#"/>
    <rdfs:comment xml:lang="en">Links a bot:Site to an instance that encodes the latitude and longitude of the Zero Point of the building site. This could be an instance of a wgs84:Point. The definition of GIS and geometry is not within the scope of BOT and an appropriate ontology needs to be selected here by the user. The use of this property is potentially ambiguous and it might be removed or revised in future editions of the ontology.</rdfs:comment>
    <rdf:type rdf:resource="http://www.w3.org/2002/07/owl#ObjectProperty"/>
  </rdf:Description>
  <rdf:Description rdf:about="https://w3id.org/bot#">
    <dcterms:issued rdf:datatype="http://www.w3.org/2001/XMLSchema#dateTime">2018-06-21T12:00:00</dcterms:issued>
    <dcterms:creator rdf:resource="https://orcid.org/0000-0002-2033-859X"/>
    <owl:priorVersion rdf:resource="https://w3id.org/bot-0.3.0"/>
    <dcterms:modified rdf:datatype="http://www.w3.org/2001/XMLSchema#dateTime">2019-07-23T12:00:00</dcterms:modified>
    <dcterms:creator rdf:resource="http://maxime-lefrancois.info/me#"/>
    <dcterms:license rdf:resource="https://creativecommons.org/licenses/by/1.0/"/>
    <dcterms:creator>Georg Ferdinand Schneider</dcterms:creator>
    <vann:preferredNamespaceUri rdf:resource="https://w3id.org/bot#"/>
    <dcterms:contributor>All contributing members of the W3C Linked Building Data Community Group</dcterms:contributor>
    <owl:versionIRI rdf:resource="https://w3id.org/bot-0.3.1"/>
    <rdfs:seeAlso rdf:resource="https://doi.org/10.24928/JC3-2017/0153"/>
    <dcterms:creator>Pieter Pauwels</dcterms:creator>
    <vann:preferredNamespacePrefix>bot</vann:preferredNamespacePrefix>
    <dcterms:creator rdf:resource="https://orcid.org/0000-0001-8020-4609"/>
    <rdfs:seeAlso rdf:resource="https://www.researchgate.net/publication/320631574_Recent_changes_in_the_Building_Topology_Ontology"/>
    <dcterms:creator>Maxime Lefrançois</dcterms:creator>
    <owl:versionInfo>0.3.1</owl:versionInfo>
    <rdf:type rdf:resource="http://purl.org/vocommons/voaf#Vocabulary"/>
    <dcterms:creator rdf:resource="https://orcid.org/0000-0002-6519-7057"/>
    <dcterms:title xml:lang="en">The Building Topology Ontology (BOT)</dcterms:title>
    <dcterms:creator>Mads Holten Rasmussen</dcterms:creator>
    <dcterms:description xml:lang="en">The Building Topology Ontology (BOT) is a simple ontology defining the core concepts of a building.
It is a simple, easy to extend ontology for the construction industry to document and exchange building data on the web.

Changes since version 0.2.0 of the ontology are documented in:

https://w3id.org/bot/bot.html#changes

The version 0.2.0 of the ontology is documented in:

Mads Holten Rasmussen, Pieter Pauwels, Maxime Lefrançois, Georg Ferdinand Schneider, Christian Anker Hviid and Jan Karlshøj (2017) Recent changes in the Building Topology Ontology, 5th Linked Data in Architecture and Construction Workshop (LDAC2017), November 13-15, 2017, Dijon, France, https://www.researchgate.net/publication/320631574_Recent_changes_in_the_Building_Topology_Ontology

The initial version 0.1.0 of the ontology was documented in:

Mads Holten Rasmussen, Pieter Pauwels, Christian Anker Hviid and Jan Karlshøj (2017) Proposing a Central AEC Ontology That Allows for Domain Specific Extensions, Lean and Computing in Construction Congress (LC3): Volume I – Proceedings of the Joint Conference on Computing in Construction (JC3), July 4-7, 2017, Heraklion, Greece, pp. 237-244 https://doi.org/10.24928/JC3-2017/0153</dcterms:description>
    <rdf:type rdf:resource="http://www.w3.org/2002/07/owl#Ontology"/>
  </rdf:Description>
  <rdf:Description rdf:about="https://w3id.org/bot#Storey">
    <owl:disjointWith rdf:resource="https://w3id.org/bot#Site"/>
    <rdfs:comment xml:lang="sv">Ett plan i en byggnad</rdfs:comment>
    <rdfs:isDefinedBy rdf:resource="https://w3id.org/bot#"/>
    <rdfs:comment xml:lang="de">Die Gesamtheit aller Räume in einem Gebäude, die auf einer Zugangsebene liegen und horizontal verbunden sind</rdfs:comment>
    <rdfs:comment xml:lang="nl">Een vlak gedeelte van een gebouw</rdfs:comment>
    <owl:disjointWith rdf:resource="https://w3id.org/bot#Building"/>
    <rdfs:label xml:lang="nl">Verdieping</rdfs:label>
    <rdfs:label xml:lang="it">Piano di edificio</rdfs:label>
    <rdfs:label xml:lang="en">Storey</rdfs:label>
    <rdfs:label xml:lang="sv">Våning</rdfs:label>
    <owl:disjointWith rdf:resource="https://w3id.org/bot#Space"/>
    <rdfs:comment xml:lang="fr">Correspond à un niveau du bâtiment</rdfs:comment>
    <rdfs:subClassOf rdf:resource="https://w3id.org/bot#Zone"/>
    <rdfs:label xml:lang="fr">Etage</rdfs:label>
    <rdfs:label xml:lang="da">Etage</rdfs:label>
    <rdfs:comment xml:lang="nl">Een horizontaal gedeelte van een gebouw</rdfs:comment>
    <vs:term_status>stable</vs:term_status>
    <rdfs:comment xml:lang="es">Un nivel de un edificio</rdfs:comment>
    <rdfs:comment xml:lang="en">A level part of a building</rdfs:comment>
    <rdfs:label xml:lang="es">Piso</rdfs:label>
    <rdfs:comment xml:lang="da">Et plan i en bygning</rdfs:comment>
    <rdfs:label xml:lang="de">Geschoss (Architektur)</rdfs:label>
    <rdf:type rdf:resource="http://www.w3.org/2002/07/owl#Class"/>
  </rdf:Description>
  <rdf:Description rdf:about="https://orcid.org/0000-0002-2033-859X">
    <schema:name>Georg Ferdinand Schneider</schema:name>
    <vcard:fn>Georg Ferdinand Schneider</vcard:fn>
    <rdf:type rdf:resource="https://schema.org/Person"/>
    <rdf:type rdf:resource="http://www.w3.org/2006/vcard/ns#Individual"/>
  </rdf:Description>
  <rdf:Description rdf:about="https://w3id.org/bot#hasSpace">
    <rdfs:label xml:lang="en">has space</rdfs:label>
    <rdfs:comment xml:lang="da">Relation til rum indeholdt i en zone. De typiske domæner for bot:hasSpace er forekomster af bot:Storey og bot:Building.</rdfs:comment>
    <rdf:type rdf:resource="http://www.w3.org/2002/07/owl#ObjectProperty"/>
    <vs:term_status>stable</vs:term_status>
    <rdfs:comment xml:lang="fr">Relation à définir entre les pièces d'une même zone. Cette propriété s'applique typiquement sur des instances de bot:Building.</rdfs:comment>
    <rdfs:label xml:lang="nl">heeft ruimte</rdfs:label>
    <rdfs:comment xml:lang="nl">Relatie tot ruimtes die zich in een zone bevinden. De typische domeinen van bot:hasSpace zijn instanties van bot:Storey en bot:Building.</rdfs:comment>
    <rdfs:label xml:lang="es">tiene espacio</rdfs:label>
    <rdfs:isDefinedBy rdf:resource="https://w3id.org/bot#"/>
    <rdfs:comment xml:lang="de">Beziehung von Räumen, die sich in einer Zone befinden. Oft ist die rdfs:domain eine Instanz von bot:Storey oder bot:Building.</rdfs:comment>
    <rdfs:domain rdf:resource="https://w3id.org/bot#Zone"/>
    <rdfs:label xml:lang="sv">har rum</rdfs:label>
    <rdfs:label xml:lang="da">har rum</rdfs:label>
    <rdfs:label xml:lang="fr">contient pièce</rdfs:label>
    <rdfs:comment xml:lang="en">Relation to spaces contained in a zone. The typical domains of bot:hasSpace are instances of bot:Storey and bot:Building.</rdfs:comment>
    <rdfs:comment xml:lang="sv">Relation till rum som inryms i en zon. Typiska domäner för bot:hasSpace är förekomster av bot:Storey och bot:Building.</rdfs:comment>
    <rdfs:comment xml:lang="es">Relación a espacios contenidos en una zona. Los dominios típicos de bot:hasSPace son instancias de bot:Storey y bot:Building.</rdfs:comment>
    <rdfs:subPropertyOf rdf:resource="https://w3id.org/bot#containsZone"/>
    <rdfs:range rdf:resource="https://w3id.org/bot#Space"/>
    <schema:domainIncludes rdf:resource="https://w3id.org/bot#Storey"/>
    <rdfs:label xml:lang="de">hat Raum</rdfs:label>
  </rdf:Description>
  <rdf:Description rdf:about="http://xmlns.com/foaf/0.1/Person">
    <rdf:type rdf:resource="http://www.w3.org/2002/07/owl#Class"/>
  </rdf:Description>
  <rdf:Description rdf:about="https://w3id.org/bot#Zone">
    <rdfs:comment xml:lang="nl">PLEASE UPDATE Een gebied of stuk land dat een dat een bepaalde karakteristiek of bestemming heeft, ergens voor gebruikt wordt of waar bepaalde restricties gelden. Een bot:Zone kan andere bot:Zones bevatten gedefinieerd door de relatie bot:containsZone, en kan verbonden zijn met andere bot:Zones gedefinieerd door de relatie bot:adjacentZone.</rdfs:comment>
    <rdfs:comment xml:lang="en">A part of the physical world or a virtual world that is inherently both located in this world and having a 3D spatial extent; Sub-classes of bot:Zone include bot:Site, bot:Building, bot:Storey, or bot:Space. An instance of bot:Zone can contain other bot:Zone instances, making it possible to group or subdivide zones. An instance of bot:Zone can be adjacent to other bot:Zone instances. Finally, a bot:Zone can instantiate two relations to bot:Element, which are either contained in (bot:containsElement), or adjacent to it (bot:adjacentElement).</rdfs:comment>
    <rdfs:comment xml:lang="fr">Une partie du monde physique ou virtuel qui est inhéremment à la fois localisé dans ce monde et a une étendue spatiale 3D; les sous-classes de bot:Zone incluent bot:Site, bot:Building, bot:Storey, ou bot:Space. Une instance de bot:Zone peut contenir d'autres instances de bot:Zone, ce qui permet de grouper ou sub-diviser les zones. Une instance de bot:Zone peut être adjacente à d'autres bot:Zone. Enfin, une bot:Zone peut contenir (bot:containsElement) our être adjacent (bot:adjacentElement) à une instance de bot:Element.</rdfs:comment>
    <rdfs:comment xml:lang="sv">PLEASE UPDATE En area eller ett stycke land som har en specifik karaktäristik, syfte, användning eller är förmål för specifika restriktioner. En bot:Zone kan innehålla andra bot:Zoner genom relationen bot:containsZone, och den kan kopplas till andra bot:Zoner genom relationen bot:adjacentZone.</rdfs:comment>
    <rdfs:label xml:lang="sv">Zon</rdfs:label>
    <rdfs:comment xml:lang="da">PLEASE UPDATE En rummelig 3D-inddeling. Underklasser af bot:Zone inkluderer bot:Site, bot:Building, bot:Storey eller bot:Space. En bot:Zone forekomst kan indeholde andre bot:Zone forekomster, hvilket gør det muligt at gruppere eller underinddele zoner. En forekomst af bot:Zone kan være tilstødende til andre bot:Zone forekomster. Endelig kan en bot:Zone instantiere to relationer til et bot:Element, hvilke er enten indeholdt i (bot:containsElement) eller tilstødende dertil (bot:adjacentElement).</rdfs:comment>
    <rdfs:label xml:lang="fr">Zone</rdfs:label>
    <rdfs:label xml:lang="de">Zone</rdfs:label>
    <rdfs:label xml:lang="da">Zone</rdfs:label>
    <rdfs:label xml:lang="es">Zona</rdfs:label>
    <rdfs:comment xml:lang="de">PLEASE UPDATE Ein abstraktes Konzept für eine räumliche, dreidimensionale Einteilung eines Raums. Spezialisierungen von bot:Zone sind bot:Site, bot:Building, bot:Storey oder bot:Space. Eine Instanz von bot:Zone kannn andere Instanzen von bot:Zone enthalten. So ist es möglich Instanzen von bot:Zone zu gruppieren, oder zu unterteilen. Eine Instanz einer bot:Zone kann an eine andere Instanz von bot:Zone angrenzen. Es bestehen zwei Möglichkeiten Instanzen von bot:Zone und bot:Element in Beziehung zu setzen. Entweder ein Element ist in einer Zone enthalten (bot:containsElement) oder es grenzt an eine andere Zone an (bot:adjacentElement).</rdfs:comment>
    <rdfs:label xml:lang="nl">Zone</rdfs:label>
    <rdfs:label xml:lang="en">Zone</rdfs:label>
    <rdf:type rdf:resource="http://www.w3.org/2002/07/owl#Class"/>
    <vs:term_status>stable</vs:term_status>
    <rdfs:comment xml:lang="es">PLEASE UPDATE Una área o espacio de tierra que tiene una característica, propósito o uso particular, o que está sujeto a restricciones particulares. Un bot:Zone puede contener otros bot:Zones definidos mediante la relación bot:containsZone, y puede estar conectado con otros bot:Zones mediante la relación bot:adjacentZone.</rdfs:comment>
    <rdfs:isDefinedBy rdf:resource="https://w3id.org/bot#"/>
    <owl:disjointWith rdf:resource="https://w3id.org/bot#Element"/>
    <owl:disjointWith rdf:resource="https://w3id.org/bot#Interface"/>
  </rdf:Description>
  <rdf:Description rdf:about="https://w3id.org/bot#Building">
    <rdfs:label xml:lang="it">Edificio</rdfs:label>
    <rdfs:label xml:lang="en">Building</rdfs:label>
    <rdfs:label xml:lang="es">Edificio</rdfs:label>
    <rdfs:comment xml:lang="en">An independent unit of the built environment with a characteristic spatial structure, intended to serve at least one function or user activity [ISO 12006-2:2013]</rdfs:comment>
    <owl:disjointWith rdf:resource="https://w3id.org/bot#Space"/>
    <rdfs:label xml:lang="sv">Byggnad</rdfs:label>
    <rdf:type rdf:resource="http://www.w3.org/2002/07/owl#Class"/>
    <rdfs:comment xml:lang="da">En uafhængig del af det byggede miljø med en karakteristisk rumlig struktur, der understøtter mindst én funktion eller brugeraktivitet</rdfs:comment>
    <rdfs:label xml:lang="da">Bygning</rdfs:label>
    <owl:disjointWith rdf:resource="https://w3id.org/bot#Site"/>
    <rdfs:label xml:lang="fr">Bâtiment</rdfs:label>
    <owl:disjointWith rdf:resource="https://w3id.org/bot#Storey"/>
    <vs:term_status>stable</vs:term_status>
    <rdfs:isDefinedBy rdf:resource="https://w3id.org/bot#"/>
    <rdfs:comment xml:lang="de">Bauwerk hauptsächlich zum Zweck des Schutzes für seine Bewohner und die darin aufbewahrten Gegenstände; im Allgemeinen teilweise oder ganz geschlossen und ortsfest [ISO 6707-1:2014]</rdfs:comment>
    <rdfs:subClassOf rdf:resource="https://w3id.org/bot#Zone"/>
    <rdfs:label xml:lang="nl">Gebouw</rdfs:label>
    <rdfs:comment xml:lang="es">Una unidad de entorno construido intependiente con una estructura espacial característica, para proporcionar al menos una función o actividad de usuario</rdfs:comment>
    <rdfs:comment xml:lang="sv">En oberoende enhet i den byggda miljön med en karaktäristisk rumslig struktur som stödjer minst en funktion eller användaraktivitet.  [ISO 12006-2:2013]</rdfs:comment>
    <rdfs:label xml:lang="de">Gebäude</rdfs:label>
    <rdfs:comment xml:lang="nl">Een onafhankelijke entiteit met een ruimtelijke structuur die onderdeel is van de gebouwde omgeving, en bedoeld is om minimaal één functie of gebruikersactiviteit te bedienen [ISO 12006-2:2013].</rdfs:comment>
    <rdfs:comment xml:lang="fr">Une unité indépendante de l'environnement bâti avec une structure spatiale caractéristique, conçue pour répondre à une fonction ou une activité de l'utilisateur [ISO 12006-2:2013]</rdfs:comment>
  </rdf:Description>
  <rdf:Description rdf:about="https://orcid.org/0000-0001-8020-4609">
    <schema:name>Pieter Pauwels</schema:name>
    <vcard:fn>Pieter Pauwels</vcard:fn>
    <rdf:type rdf:resource="https://schema.org/Person"/>
    <rdf:type rdf:resource="http://www.w3.org/2006/vcard/ns#Individual"/>
  </rdf:Description>
  <rdf:Description rdf:about="http://maxime-lefrancois.info/me#">
    <schema:name>Maxime Lefrançois</schema:name>
    <vcard:fn>Maxime Lefrançois</vcard:fn>
    <rdf:type rdf:resource="https://schema.org/Person"/>
    <rdf:type rdf:resource="http://www.w3.org/2006/vcard/ns#Individual"/>
  </rdf:Description>
  <rdf:Description rdf:about="http://purl.org/dc/terms/modified">
    <rdf:type rdf:resource="http://www.w3.org/2002/07/owl#AnnotationProperty"/>
  </rdf:Description>
  <rdf:Description rdf:nodeID="A3">
    <rdf:rest rdf:nodeID="A1"/>
    <rdf:first rdf:resource="https://w3id.org/bot#containsZone"/>
  </rdf:Description>
  <rdf:Description rdf:about="https://w3id.org/bot#containsElement">
    <rdfs:comment xml:lang="es">Relación a un elemento arquitectónico contenido en una zona.</rdfs:comment>
    <rdfs:comment xml:lang="de">Beziehung einer Zone zu einem Bauteil, dass es enthält.</rdfs:comment>
    <rdfs:label xml:lang="fr">contient élément</rdfs:label>
    <rdfs:label xml:lang="es">contiene elemento</rdfs:label>
    <rdfs:comment xml:lang="nl">Relatie tussen zone en een gebouwelement in die zone</rdfs:comment>
    <rdfs:label xml:lang="en">contains element</rdfs:label>
    <rdfs:comment xml:lang="da">Relation til en bygningsdel, som er indeholdt i en zone.</rdfs:comment>
    <owl:propertyChainAxiom rdf:nodeID="A3"/>
    <rdfs:label xml:lang="nl">bevat element</rdfs:label>
    <rdfs:comment xml:lang="fr">Relation à définir entre un élément de bâti et la zone le contenant</rdfs:comment>
    <rdf:type rdf:resource="http://www.w3.org/2002/07/owl#ObjectProperty"/>
    <vs:term_status>stable</vs:term_status>
    <rdfs:isDefinedBy rdf:resource="https://w3id.org/bot#"/>
    <rdfs:subPropertyOf rdf:resource="https://w3id.org/bot#hasElement"/>
    <rdfs:label xml:lang="de">enthält Bauteil</rdfs:label>
    <rdfs:label xml:lang="sv">innehåller byggdel</rdfs:label>
    <rdfs:comment xml:lang="sv">Relation till en byggdel som inryms i en zon.</rdfs:comment>
    <rdfs:label xml:lang="da">indeholder bygningsdel</rdfs:label>
    <rdfs:comment xml:lang="en">Relation to a building element contained in a zone.</rdfs:comment>
  </rdf:Description>
  <rdf:Description rdf:about="http://www.w3.org/2003/06/sw-vocab-status/ns#term_status">
    <rdf:type rdf:resource="http://www.w3.org/2002/07/owl#AnnotationProperty"/>
  </rdf:Description>
  <rdf:Description rdf:about="http://purl.org/dc/terms/description">
    <rdf:type rdf:resource="http://www.w3.org/2002/07/owl#AnnotationProperty"/>
  </rdf:Description>
  <rdf:Description rdf:about="https://w3id.org/bot#containsZone">
    <schema:rangeIncludes rdf:resource="https://w3id.org/bot#Site"/>
    <rdfs:isDefinedBy rdf:resource="https://w3id.org/bot#"/>
    <rdf:type rdf:resource="http://www.w3.org/2002/07/owl#ObjectProperty"/>
    <rdfs:label xml:lang="sv">innehåller zon</rdfs:label>
    <rdfs:comment xml:lang="en">Relationship to the subzones of a major zone. A space zone could for instance be contained in a storey zone which is further contained in a building zone. bot:containsZone is a transitive property. This implies that in the previous example a bot:containsZone relationship holds between the space zone and the building zone.</rdfs:comment>
    <rdfs:label xml:lang="nl">bevat zone</rdfs:label>
    <schema:rangeIncludes rdf:resource="https://w3id.org/bot#Building"/>
    <rdf:type rdf:resource="http://www.w3.org/2002/07/owl#TransitiveProperty"/>
    <rdfs:comment xml:lang="de">Beziehung zwischen Zonen, wobei eine die andere enthält. Zum Beispiel kann eine Raumzone in einer Geschossszone enthalten sein, die wiederrum in einer Gebäudezone enthalten ist. bot:containsZone is eine transitive Beziehung, dass heisst zwischen der Raumzone im vorherigen Beispiel und der Gebäudezone besteht auch die Beziehung bot:containsZone.</rdfs:comment>
    <vs:term_status>stable</vs:term_status>
    <rdfs:domain rdf:resource="https://w3id.org/bot#Zone"/>
    <rdfs:label xml:lang="es">contiene zona</rdfs:label>
    <schema:domainIncludes rdf:resource="https://w3id.org/bot#Space"/>
    <rdfs:comment xml:lang="da">Relation til underzoner i en større zone. En rum-zone kan for eksempel være indeholdt i en etage-zone som ydermere er indeholdt i en bygnings-zone. bot:containsZone er en transitiv egenskab, hvilket betyder at rum-zonen i det forrige eksempel også er indeholdt i bygnings-zonen.</rdfs:comment>
    <schema:domainIncludes rdf:resource="https://w3id.org/bot#Site"/>
    <rdfs:label xml:lang="da">indeholder zone</rdfs:label>
    <rdfs:label xml:lang="en">contains zone</rdfs:label>
    <schema:rangeIncludes rdf:resource="https://w3id.org/bot#Storey"/>
    <rdfs:label xml:lang="fr">contient zone</rdfs:label>
    <rdfs:comment xml:lang="sv">Relation till delzoner i en huvudzon. En rumszon kan till exempel inrymmas i en våningszon som i sin tur inryms i en byggnadszon. bot:containsZone är en transitiv relation vilket i exemplet betyder att rumszonen också inryms i byggnadszonen.</rdfs:comment>
    <schema:rangeIncludes rdf:resource="https://w3id.org/bot#Space"/>
    <schema:domainIncludes rdf:resource="https://w3id.org/bot#Storey"/>
    <rdfs:range rdf:resource="https://w3id.org/bot#Zone"/>
    <schema:domainIncludes rdf:resource="https://w3id.org/bot#Building"/>
    <rdfs:comment xml:lang="fr">Relation entre les sous-zones composant une zone plus grande. Cette propriété est transitive.</rdfs:comment>
    <rdfs:label xml:lang="de">enthält Zone</rdfs:label>
    <rdfs:comment xml:lang="nl">Relatie tussen subzones van een hoofd zone. Een ruimtezone kan bijvoorbeeld worden bevat door een verdiepingszone, die wederom bevat wordt door een gebouwzone. bot:containsZone is een transitieve eigenschap, wat betekent dat in het vorige voorbeeld de ruimtezone ook bevat wordt door de gebouwzone.</rdfs:comment>
  </rdf:Description>
  <rdf:Description rdf:about="http://purl.org/dc/terms/issued">
    <rdf:type rdf:resource="http://www.w3.org/2002/07/owl#AnnotationProperty"/>
  </rdf:Description>
  <rdf:Description rdf:about="http://purl.org/vocab/vann/preferredNamespaceUri">
    <rdf:type rdf:resource="http://www.w3.org/2002/07/owl#AnnotationProperty"/>
  </rdf:Description>
  <rdf:Description rdf:about="https://w3id.org/bot#Space">
    <rdfs:label xml:lang="sv">Utrymme</rdfs:label>
    <rdfs:label xml:lang="da">Rum</rdfs:label>
    <rdfs:label xml:lang="nl">Ruimte</rdfs:label>
    <rdfs:comment xml:lang="fr">Une partie du monde physique ou virtuel dont l'extension 3D est limitée réellement ou théoriquement, et apporte des fonctions aux zones dans laquelle elle est contenue.</rdfs:comment>
    <rdfs:label xml:lang="es">Espacio</rdfs:label>
    <rdfs:label xml:lang="fr">Pièce</rdfs:label>
    <rdfs:comment xml:lang="sv">PLEASE UPDATE En avgränsad tredimensionell utsträckning som definierats fysiskt eller fiktivt [ISO 12006-2 (DIS 2013), 3.4.3]</rdfs:comment>
    <owl:disjointWith rdf:resource="https://w3id.org/bot#Building"/>
    <rdfs:label xml:lang="it">Spazio</rdfs:label>
    <owl:disjointWith rdf:resource="https://w3id.org/bot#Site"/>
    <rdfs:subClassOf rdf:resource="https://w3id.org/bot#Zone"/>
    <rdfs:comment xml:lang="da">PLEASE UPDATE En afgrænset tredimensionel udstrækning defineret fysisk eller fiktivt</rdfs:comment>
    <rdfs:label xml:lang="de">Raum</rdfs:label>
    <vs:term_status>stable</vs:term_status>
    <rdfs:isDefinedBy rdf:resource="https://w3id.org/bot#"/>
    <rdf:type rdf:resource="http://www.w3.org/2002/07/owl#Class"/>
    <rdfs:comment xml:lang="de">PLEASE UPDATE Fläche oder Volumen mit tatsächlicher oder theoretischer Begrenzung [ISO 6707-1:2014]</rdfs:comment>
    <owl:disjointWith rdf:resource="https://w3id.org/bot#Storey"/>
    <rdfs:comment xml:lang="nl">PLEASE UPDATE Een afgebakende driedimensionale omgeving die fysiek of indirect gedefinieerd wordt [ISO 12006-2 (DIS 2013), 3.4.3]</rdfs:comment>
    <rdfs:comment xml:lang="en">A part of the physical world or a virtual world whose 3D spatial extent is bounded actually or theoretically, and provides for certain functions within the zone it is contained in.</rdfs:comment>
    <rdfs:comment xml:lang="es">PLEASE UPDATE Una extensión tridimensional limitada y definida fisica o teóricamente</rdfs:comment>
    <rdfs:label xml:lang="en">Space</rdfs:label>
  </rdf:Description>
  <rdf:Description rdf:about="https://w3id.org/bot#interfaceOf">
    <rdfs:isDefinedBy rdf:resource="https://w3id.org/bot#"/>
    <rdfs:comment xml:lang="nl">Relatie tussen een interface en een aanliggende zone of element.</rdfs:comment>
    <rdfs:comment xml:lang="sv">Relation mellan ett gränssnitt och en angränsande zon eller byggdel.</rdfs:comment>
    <rdfs:label xml:lang="en">interface of</rdfs:label>
    <rdfs:label xml:lang="de">Grenzfläche von</rdfs:label>
    <rdfs:label xml:lang="da">grænseflade for</rdfs:label>
    <vs:term_status>stable</vs:term_status>
    <rdfs:domain rdf:resource="https://w3id.org/bot#Interface"/>
    <rdfs:label xml:lang="nl">interface van</rdfs:label>
    <rdfs:comment xml:lang="da">Relation mellem en grænseflade og en tilstødende zone eller bygningsdel.</rdfs:comment>
    <rdfs:comment xml:lang="de">Beziehung zwischen einer Grenzfläche und einer angrenzenden Zone oder einem Bauteil.</rdfs:comment>
    <rdfs:label xml:lang="fr">interface de</rdfs:label>
    <rdfs:comment xml:lang="fr">Relation à définir entre une interface et une zone ou un élément adjacents.</rdfs:comment>
    <rdfs:comment xml:lang="en">Relationship between an interface and an adjacent zone or element.</rdfs:comment>
    <rdfs:label xml:lang="sv">gränssnitt för</rdfs:label>
    <rdf:type rdf:resource="http://www.w3.org/2002/07/owl#ObjectProperty"/>
  </rdf:Description>
  <rdf:Description rdf:about="https://w3id.org/bot#adjacentElement">
    <rdfs:comment xml:lang="de">Beziehung zwischen einer Zone und dessen angrenzenden Bauteilen. Die Bauteile begrenzen die Zone.</rdfs:comment>
    <rdfs:label xml:lang="da">tilstødende element</rdfs:label>
    <rdfs:label xml:lang="sv">angränsande element</rdfs:label>
    <rdf:type rdf:resource="http://www.w3.org/2002/07/owl#ObjectProperty"/>
    <rdfs:label xml:lang="en">adjacent element</rdfs:label>
    <rdfs:comment xml:lang="da">Relation mellem en zone og dens tilstødende bygningsdele, som afgrænser det fysiske rum.</rdfs:comment>
    <rdfs:comment xml:lang="en">Relation between a zone and its adjacent building elements, bounding the zone.</rdfs:comment>
    <rdfs:comment xml:lang="sv">Relation mellan en zon och dess angränsande byggdelar, som avgränsar det fysiska utrymmet.</rdfs:comment>
    <owl:propertyDisjointWith rdf:resource="https://w3id.org/bot#intersectingElement"/>
    <rdfs:subPropertyOf rdf:resource="https://w3id.org/bot#hasElement"/>
    <rdfs:comment xml:lang="nl">Relatie tussen een zone en zijn aangrenzende gebouwelementen, begrensd door fysieke ruimte.</rdfs:comment>
    <rdfs:comment xml:lang="fr">Relation entre une zone et ses éléments adjacents, délimitant l'espace physique</rdfs:comment>
    <rdfs:label xml:lang="es">elemento adyacente</rdfs:label>
    <vs:term_status>stable</vs:term_status>
    <rdfs:label xml:lang="de">benachbartes Bauteil</rdfs:label>
    <rdfs:isDefinedBy rdf:resource="https://w3id.org/bot#"/>
    <rdfs:comment xml:lang="es">Relación entre una zona y sus elementos arquitectónicos adyacentes, que limitan el espacio físico.</rdfs:comment>
    <rdfs:label xml:lang="nl">aangrenzend element</rdfs:label>
    <rdfs:label xml:lang="fr">élément adjacent</rdfs:label>
  </rdf:Description>
  <rdf:Description rdf:about="https://w3id.org/bot#hasSimple3DModel">
    <rdfs:label xml:lang="da">har simpel 3D-model</rdfs:label>
    <rdfs:label xml:lang="en">has Simple 3D Model</rdfs:label>
    <vs:term_status>unstable</vs:term_status>
    <schema:domainIncludes rdf:resource="https://w3id.org/bot#Zone"/>
    <rdfs:comment xml:lang="de">Verbindet jede bot:Zone oder bot:Element zu einem 3D Model, dass als Literal codiert ist.</rdfs:comment>
    <rdfs:comment xml:lang="da">Forbinder enhver instans af bot:Zone eller bot:Element med en 3D-model beskrevet som en literal.</rdfs:comment>
    <schema:domainIncludes rdf:resource="https://w3id.org/bot#Element"/>
    <rdfs:label xml:lang="de">hat einfaches 3D Modell</rdfs:label>
    <rdfs:isDefinedBy rdf:resource="https://w3id.org/bot#"/>
    <rdfs:comment xml:lang="en">Links any bot:Zone or bot:Element to a 3D Model encoded as a literal.</rdfs:comment>
    <rdf:type rdf:resource="http://www.w3.org/2002/07/owl#DatatypeProperty"/>
  </rdf:Description>
  <rdf:Description rdf:nodeID="A2">
    <rdf:rest rdf:nodeID="A0"/>
    <rdf:first rdf:resource="https://w3id.org/bot#containsZone"/>
  </rdf:Description>
  <rdf:Description rdf:about="https://w3id.org/bot#adjacentZone">
    <rdfs:label xml:lang="da">tilstødende zone</rdfs:label>
    <schema:domainIncludes rdf:resource="https://w3id.org/bot#Storey"/>
    <rdfs:comment xml:lang="sv">Relation mellan två zoner som delar ett gemensamt gränssnitt.</rdfs:comment>
    <schema:rangeIncludes rdf:resource="https://w3id.org/bot#Site"/>
    <schema:domainIncludes rdf:resource="https://w3id.org/bot#Site"/>
    <rdfs:comment xml:lang="da">Relation mellem to zoner, der deler en fælles grænseflade.</rdfs:comment>
    <schema:domainIncludes rdf:resource="https://w3id.org/bot#Space"/>
    <schema:rangeIncludes rdf:resource="https://w3id.org/bot#Space"/>
    <rdfs:domain rdf:resource="https://w3id.org/bot#Zone"/>
    <rdfs:label xml:lang="en">adjacent zone</rdfs:label>
    <rdfs:label xml:lang="fr">zone adjacente</rdfs:label>
    <rdfs:label xml:lang="nl">aangrenzende zone</rdfs:label>
    <rdf:type rdf:resource="http://www.w3.org/2002/07/owl#SymmetricProperty"/>
    <rdfs:label xml:lang="es">zona adyacente</rdfs:label>
    <rdfs:isDefinedBy rdf:resource="https://w3id.org/bot#"/>
    <rdfs:comment xml:lang="fr">Relation entre deux zones partageant une interface commune, sans intersection</rdfs:comment>
    <schema:rangeIncludes rdf:resource="https://w3id.org/bot#Storey"/>
    <rdfs:comment xml:lang="de">Beziehung zwischen zwei Zonen die eine gemeinsame Grenzfläche haben, aber sich nicht schneiden.</rdfs:comment>
    <owl:propertyDisjointWith rdf:resource="https://w3id.org/bot#intersectsZone"/>
    <rdf:type rdf:resource="http://www.w3.org/2002/07/owl#ObjectProperty"/>
    <rdfs:comment xml:lang="en">Relationship between two zones that share a common interface, but do not intersect.</rdfs:comment>
    <vs:term_status>stable</vs:term_status>
    <schema:domainIncludes rdf:resource="https://w3id.org/bot#Building"/>
    <schema:rangeIncludes rdf:resource="https://w3id.org/bot#Building"/>
    <rdfs:comment xml:lang="nl">Relatie tussen twee zones die een interface delen</rdfs:comment>
    <rdfs:label xml:lang="sv">angränsande zon</rdfs:label>
    <rdfs:label xml:lang="de">angrenzende Zone</rdfs:label>
    <rdfs:range rdf:resource="https://w3id.org/bot#Zone"/>
  </rdf:Description>
  <rdf:Description rdf:about="https://w3id.org/bot#intersectingElement">
    <rdf:type rdf:resource="http://www.w3.org/2002/07/owl#ObjectProperty"/>
    <rdfs:comment xml:lang="en">Relation between a Zone and a building Element that intersects it. </rdfs:comment>
    <rdfs:isDefinedBy rdf:resource="https://w3id.org/bot#"/>
    <rdfs:label xml:lang="de">schneidendes Bauteil</rdfs:label>
    <vs:term_status>stable</vs:term_status>
    <owl:propertyDisjointWith rdf:resource="https://w3id.org/bot#adjacentElement"/>
    <rdfs:subPropertyOf rdf:resource="https://w3id.org/bot#hasElement"/>
    <rdfs:label xml:lang="fr">élément intersectant</rdfs:label>
    <rdfs:label xml:lang="en">intersecting element</rdfs:label>
    <rdfs:comment xml:lang="de">Beziehung zwischen einer Zone und einem Bauteil, das die Zone schneidet.</rdfs:comment>
  </rdf:Description>
  <rdf:Description rdf:about="http://purl.org/dc/terms/license">
    <rdf:type rdf:resource="http://www.w3.org/2002/07/owl#AnnotationProperty"/>
  </rdf:Description>
  <rdf:Description rdf:about="http://purl.org/dc/terms/title">
    <rdf:type rdf:resource="http://www.w3.org/2002/07/owl#AnnotationProperty"/>
  </rdf:Description>
  <rdf:Description rdf:about="https://w3id.org/bot#hasBuilding">
    <vs:term_status>stable</vs:term_status>
    <rdfs:label xml:lang="sv">har byggnad</rdfs:label>
    <schema:domainIncludes rdf:resource="https://w3id.org/bot#Site"/>
    <rdfs:domain rdf:resource="https://w3id.org/bot#Zone"/>
    <rdfs:label xml:lang="da">har bygning</rdfs:label>
    <rdfs:comment xml:lang="de">Beziehung zwischen Gebäuden, die in einer Zone enthalten sind. Oft ist hier die rdfs:domain eine Instanz von bot:Site.</rdfs:comment>
    <rdfs:isDefinedBy rdf:resource="https://w3id.org/bot#"/>
    <rdfs:comment xml:lang="fr">Relation à définir entre les bâtiments d'une même zone. Cette propriété s'applique typiquement sur des instances de bot:Site.</rdfs:comment>
    <rdfs:range rdf:resource="https://w3id.org/bot#Building"/>
    <rdfs:label xml:lang="es">tiene edificio</rdfs:label>
    <rdfs:subPropertyOf rdf:resource="https://w3id.org/bot#containsZone"/>
    <rdfs:label xml:lang="fr">contient bâtiment</rdfs:label>
    <rdfs:comment xml:lang="sv">Relation till byggnader som inryms i en zon. Typiska domäner för bot:hasBuilding är förekomster av bot:Site.</rdfs:comment>
    <rdfs:comment xml:lang="nl">Relatie tot gebouwen die zich op een terrein bevinden</rdfs:comment>
    <rdf:type rdf:resource="http://www.w3.org/2002/07/owl#ObjectProperty"/>
    <rdfs:label xml:lang="en">has building</rdfs:label>
    <rdfs:comment xml:lang="da">Relation til bygninger indeholdt i en zone. De typiske domæner for bot:hasBuilding er forekomster af bot:Site.</rdfs:comment>
    <rdfs:label xml:lang="nl">heeft gebouw</rdfs:label>
    <rdfs:comment xml:lang="en">Relation to buildings contained in a zone. The typical domains of bot:hasBuilding are instances of bot:Site.</rdfs:comment>
    <rdfs:label xml:lang="de">hat Gebäude</rdfs:label>
  </rdf:Description>
</rdf:RDF>
